

\[AV_{m-1}=V_m H_{m,m-1}
=[v_1,\ldots,v_m]
\begin{bmatrix}
    h_{1,1} & h_{1,2} & \ldots & h_{1,m-2} & h_{1,m-1}\\
    h_{2,1} & h_{2,2} & & h_{2,m-2} & h_{2,m-1} \\
    0 & h_{3,2} & & h_{3,m-2} & h_{3,m-1} \\ 
    \vdots & & \ddots & \vdots &\vdots\\
    & & & h_{m-1,m-2} & h_{m-1,m-1}\\
    0 & & \ldots  & 0 & h_{m,m-1}
\end{bmatrix}\]

\[=\left[\sum_{i=1}^{2}h_{i,1}v_i,\quad\sum_{i=1}^{3}h_{i,2}v_i,
\quad\ldots,\sum_{i=1}^{m-1}h_{i,m-2}v_i, \quad \sum_{i=1}^{m}h_{i,m-1}v_i\right]\]

\[=\left[\sum_{i=1}^{2}h_{i,1}v_i,\quad\sum_{i=1}^{3}h_{i,2}v_i,
\quad\ldots,\sum_{i=1}^{m-1}h_{i,m-2}v_i, \quad \sum_{i=1}^{m-1}h_{i,m-1}v_i\right]
+h_{m,m-1}v_m e_{m-1}^T\]
\[=V_{m-1} H_{m-1,m-1}+h_{m,m-1}v_m e^T_{m-1}\]





\[V^T_{m-1}AV_{m-1}=V^T_{m-1}V_{m-1} H_{m-1,m-1}+h_{m,m-1}V^T_{m-1}v_m e^T_{m-1}\]
\[V^T_{m-1}AV_{m-1}=IH_{m-1,m-1}+0=H_{m-1,m-1}\]


\[AV_{m-1}=V_{m-1}H_{m-1,m-1}\]
